Most of the proofs finished except Full-Adder

src/Utility.lean
@@ -1,16 +1,27 @@
 import data.vector tactic Gates
 
+def stream (α : Type) := ℕ → α
+
+def signal := ℕ → bool
+
+def sig_n (n : ℕ) := ℕ → array n bool
+
+def sig_n_zero (n : ℕ) : sig_n n := λ t, mk_array n ff
+
+def sig_tt : signal := λ t, tt
+def sig_ff : signal := λ t, ff
+
 def bool_to_nat : bool → ℕ 
   | tt := 1
   | ff := 0
---bewijs
+
 def nat_to_bool : ℕ → bool
   | nat.zero := ff
   | (nat.succ _) := tt
 
 def bool_arr_to_nat {n : ℕ} (v : array n bool) : ℕ :=
   let acc := 0 in
-  v.foldl acc (λ b acc, cond b (2 * acc + 1) (2 * acc + 0))
+  v.foldl acc (λ b acc, nat.bit b acc)
 
 def zip_array {n : ℕ} {α β : Type} (a : array n α) (b : array n β) : array n (α × β) :=
   ⟨λ i, (a.read i, b.read i)⟩
@@ -30,16 +41,39 @@ def fold_array {n : ℕ} {α β γ δ : Type} (f : α → β → γ → (δ × �
   let acc := i in
   fold_array_aux f a n (le_refl _) acc
 
-def fold_lsh_aux {n : ℕ} {α β γ: Type} (f : α → β → (γ × β)) (a : array n α) : 
-                    Π (i : ℕ), i ≤ n → (array n γ × β) → (array n γ × β) 
-| nat.zero     h acc := acc
-| (nat.succ j) h acc :=
-  let i : fin n := ⟨j, h⟩,
-    (res, next) := f (a.read i) acc.snd in
-    fold_lsh_aux j (le_of_lt h) (acc.fst.write i res, next)
 
-def fold_lsh {n : ℕ} {α β γ : Type} (f : α → β → (γ × β)) (a : array n α) 
-								(i : array n γ × β) : (array n γ) :=
-  let acc := i in
-  (fold_lsh_aux f a n (le_refl _) acc).fst
+lemma zip_unzip_eq {n : ℕ} {α β : Type} (a : array n α) (b : array n β) :
+  unzip_array (zip_array a b) = (a, b) :=
+  begin
+    unfold zip_array unzip_array,
+    simp,
+    split,
+    {
+      apply array.ext,
+      intros i,
+      apply array.read_map,
+    },
+    {
+      apply array.ext,
+      intros i,
+      apply array.read_map,
+    }
+  end
 
+lemma unzip_zip_eq {n : ℕ} {α β : Type} (a : array n (α × β)) :
+  zip_array (unzip_array a).fst (unzip_array a).snd = a :=
+  begin
+    unfold zip_array unzip_array,
+    simp,
+    apply array.ext,
+    intros i,
+    exact prod.ext rfl rfl,
+  end
+
+
+def nat_to_bool_list (n : ℕ) : list bool :=
+n.binary_rec [] (λ b n l, (b :: l))
+
+def nat_to_bool_list_rev : ℕ → list bool
+| 0 := [ff]
+| n := list.reverse (nat_to_bool_list n)
