src/Adder.lean
@@ -1,0 +1,85 @@
+import Utility
+
+def full_adder_spec (A B Cin Sum Cout : bool) : Prop :=
+	Sum = nat_to_bool ((bool_to_nat A + bool_to_nat B + bool_to_nat Cin) % 2) ∧ --sum
+	Cout = ((bool_to_nat A + bool_to_nat B + bool_to_nat Cin) ≥ 2) --carry out
+
+theorem full_adder_unique : ∀ (A B CIN : bool), ∃!(SUM : bool), ∃(COUT : bool),
+  full_adder_spec A B CIN SUM COUT :=
+  begin
+    intros A B CIN,
+    apply exists_unique_of_exists_of_unique,
+    {
+      unfold full_adder_spec,
+      simp,
+      cases A; cases B; cases CIN;
+      {
+        unfold bool_to_nat nat_to_bool,
+        simp,
+        unfold nat_to_bool,
+        simp,
+      }
+    },
+    {
+      intros y₁ y₂,
+      unfold full_adder_spec,
+      simp,
+      intros h₁ h₂,
+      finish,
+    }
+  end
+
+--returns (sum x cout)
+def full_adder_imp (A B Cin : bool) : (bool × bool) :=
+	let p := XOR [A, B],
+			q := AND [Cin, p],
+			r := AND [A, B] in
+	(XOR [p, Cin], OR [q, r])
+
+
+theorem full_adder_correct : ∀ (A B CIN : bool), ∀ (SUM COUT : bool), 
+  full_adder_spec A B CIN SUM COUT ↔ full_adder_imp A B CIN = (SUM, COUT) :=
+  begin
+    intros,
+    unfold full_adder_imp full_adder_spec,
+    simp,
+    cases A; cases B; cases CIN;
+    {
+      unfold bool_to_nat AND OR XOR,
+      simp,
+      unfold nat_to_bool,
+      tautology,
+    }
+  end 
+
+def full_n_adder_imp {n : ℕ} (A B : array n bool) (Cin : bool) : (array n bool × bool) :=
+		fold_array (full_adder_imp) (zip_array A B) (mk_array n ff, Cin)
+
+def full_n_adder_spec {n : ℕ} (A B : array n bool) (Cin : bool) (Sum : array n bool) (Cout : bool) : Prop :=
+		bool_arr_to_nat Sum = ((bool_arr_to_nat A + bool_arr_to_nat B + bool_to_nat Cin) % 2^n) ∧
+		Cout = ((bool_arr_to_nat A + bool_arr_to_nat B + bool_to_nat Cin) ≥ 2^n)
+
+theorem full_n_adder_unique {n : ℕ} : ∀ (A B SUM : array n bool)(CIN : bool), ∃!(SUM : array n bool), ∃(COUT : bool),
+  full_n_adder_spec A B CIN SUM COUT :=
+  begin
+    intros A B SUM CIN,
+    apply exists_unique_of_exists_of_unique,
+    {
+      unfold full_n_adder_spec,
+      simp,
+      unfold bool_arr_to_nat,
+      simp,
+      sorry,
+    },
+    {
+      intros y₁ y₂,
+      unfold full_n_adder_spec,
+      simp,
+      intros h₁ h₂,
+      finish,
+    }
+  end
+
+
+
+
