src/Memory.lean
@@ -1,0 +1,132 @@
+import Utility tactic 
+
+def mem_spec {α : Type} (D : stream α) (S : signal) (M : stream α) : Prop :=
+  ∀ t : ℕ,
+    (S t = tt → M (t+1) = D t) ∧  --frame 1 D S M+1
+    (S t = ff → M (t+1) = M t)    --frame 2 S M M+1
+
+def almost_eq {α : Type} (N M : stream α) : Prop :=
+  ∀ (t : ℕ),
+    (N t = M t) → ∀ (t' : ℕ), (t' > t) → N t' = M t'
+
+def almost_eq' {α : Type} (N M : stream α) : Prop :=
+  ∀ (t : ℕ),
+    (N t = M t) → N (t+1) = M (t+1)
+
+lemma almost_eq_equiv {α : Type} (N M : stream α) : almost_eq N M ↔ almost_eq' N M :=
+  begin
+    unfold almost_eq almost_eq',
+    split,
+    {
+      intros h t,
+      specialize h t,
+      intros h₁,
+      apply h,
+      {
+        exact h₁,
+      },
+      {
+        simp,
+      }
+    },
+    {
+      sorry, --almost_eq too strong
+    }
+  end
+
+theorem mem_spec_almost_unique {α : Type} : ∀ (D : stream α) (S : signal) (M : stream α),
+  mem_spec D S M → ∀(N : stream α), mem_spec D S N → almost_eq' N M :=
+  begin
+    intros D S M h₁ N h₂,
+    unfold almost_eq',
+    intros t heq,
+    unfold mem_spec at h₁ h₂,
+    specialize h₁ t,
+    specialize h₂ t,
+    destruct h₁,
+    intros h₁l h₁r,
+    destruct h₂,
+    intros h₂l h₂r,
+    cases S t,
+    {
+      simp at h₂r,
+      rw h₂r,
+      simp at h₁r,
+      rw h₁r,
+      exact heq,
+    },
+    {
+      simp at h₂l,
+      rw h₂l,
+      simp at h₁l,
+      rw h₁l,
+    }
+  end
+
+def mem_imp (I: bool) (D S: signal) : signal
+  | nat.zero := I
+  | (nat.succ y) := if S y = tt then D y 
+                    else mem_imp y
+
+def mem_n_imp {n : ℕ} (I : array n bool) (D : sig_n n) (S : signal) : sig_n n
+  | nat.zero := I
+  | (nat.succ y) := if S y = tt then D y
+                    else mem_n_imp y
+
+theorem mem_correct : ∀ (D S : signal), ∀ (I : bool),
+  mem_spec D S (mem_imp I D S) :=
+  begin
+    intros D S I,
+    unfold mem_spec,
+    intro t,
+    split,
+    {
+      intros h,
+      unfold mem_imp,
+      simp,
+      intro h',
+      exfalso,
+      rewrite h at h',
+      simp at h',
+      assumption,
+    },
+    {
+      intros h,
+      unfold mem_imp,
+      simp,
+      intro h',
+      exfalso,
+      rewrite h at h',
+      simp at h',
+      assumption,
+    }
+  end
+
+theorem mem_n_correct {n : ℕ} : ∀ (D : sig_n n) (S: signal),
+  mem_spec D S (mem_n_imp (mk_array n ff) D S) :=
+  begin
+    unfold mem_spec,
+    intros,
+    split,
+    {
+      intros h,
+      unfold mem_n_imp,
+      simp, --rewrite if_pos,
+      intro h', -- exact h,
+      exfalso,
+      rewrite h at h',
+      simp at h',
+      assumption,
+    },
+    {
+      intros h,
+      unfold mem_n_imp,
+      simp,
+      intro h',
+      exfalso,
+      rewrite h at h',
+      simp at h',
+      assumption,
+    },
+  end
+
