src/PC.lean
@@ -1,0 +1,33 @@
+import Utility Adder
+
+def pc_spec {n : ℕ} (R : signal) (O : sig_n n) : Prop :=
+  ∀ t : ℕ,
+    (R t = tt → O (nat.succ t) = mk_array n ff) ∧
+    (R t = ff → O (nat.succ t) = (full_n_adder_imp (O t) (mk_array n ff) tt).fst)
+
+def pc_imp {n : ℕ} (I : array n bool) (R : signal) : sig_n n
+  | nat.zero := I
+  | (nat.succ y) := if R y = tt then I
+                    else (full_n_adder_imp (pc_imp y) (mk_array n ff) (tt)).fst
+
+theorem pc_correct {n : ℕ} : ∀ (R : signal) (I : array n bool),
+  pc_spec R (pc_imp (mk_array n ff) R) :=
+  begin
+    intros,
+    unfold pc_spec,
+    intros t,
+    split,
+    {
+      intros h₁,
+      unfold pc_imp,
+      rw if_pos,
+      exact h₁,
+    },
+    {
+      intros h₁,
+      unfold pc_imp,
+      rw if_neg,
+      simp,
+      exact h₁, 
+    }
+  end
