src/SeqRec.lean
@@ -1,0 +1,159 @@
+import Utility tactic
+
+--Logic Unit 2
+def LUT2 (Q1 Q0 X : bool) : bool :=
+  OR [AND [Q1, Q0, X], AND [Q1, NOT Q0 , X], AND[NOT Q1, Q0, X], AND[NOT Q1, NOT Q0, X]]
+
+def LUT2_spec (Q1 Q0 X OUT : bool) : Prop :=
+  if (¬Q1 ∧ ¬Q0 ∧ X) ∨ (¬Q1 ∧ Q0 ∧ X) ∨ (Q1 ∧ ¬Q0 ∧ X) ∨ (Q1 ∧ Q0 ∧ X) then OUT = tt
+  else OUT = ff
+
+theorem LUT2_correct : ∀ (Q1 Q0 X : bool),
+  ∀ (OUT : bool), LUT2_spec Q1 Q0 X OUT ↔ LUT2 Q1 Q0 X  = OUT :=
+  begin
+    intros,
+    unfold LUT2_spec LUT2,
+    cases Q1; cases Q0; cases X;
+    {
+      unfold AND OR NOT,
+      simp,
+      rw eq_comm,
+    }
+  end
+
+--Logic Unit 3
+def LUT3 (Q1 Q0 X : bool) : bool :=
+  OR [AND [NOT Q1, Q0, NOT X], AND [Q1, NOT Q0 , X], AND [Q1, Q0, X]]
+
+
+def LUT3_spec (Q1 Q0 X OUT : bool) : Prop :=
+  if (¬Q1 ∧ Q0 ∧ ¬X) ∨ (Q1 ∧ ¬Q0 ∧ X) ∨ (Q1 ∧ Q0 ∧ X) then OUT = tt
+  else OUT = ff
+
+theorem LUT3_correct : ∀ (Q1 Q0 X : bool),
+  ∀ (OUT : bool), LUT3_spec Q1 Q0 X OUT ↔ LUT3 Q1 Q0 X  = OUT :=
+  begin
+    intros,
+    unfold LUT3_spec LUT3,
+    cases Q1; cases Q0; cases X;
+    {
+      unfold AND OR NOT,
+      simp,
+      rw eq_comm,
+    }
+  end
+
+--Logic Unit 0
+def LUT0 (Q1 Q0 : bool) : bool :=
+  AND[Q1, Q0]
+
+def LUT0_spec (Q1 Q0 OUT : bool) :=
+  if Q1 ∧ Q0 then OUT = tt else OUT = ff
+
+theorem LUT0_correct : ∀ (Q1 Q0 : bool), ∀ (OUT : bool),
+  LUT0_spec Q1 Q0 OUT ↔ LUT0 Q1 Q0 = OUT :=
+  begin
+    intros,
+    unfold LUT0_spec LUT0,
+    cases Q1; cases Q0;
+    {
+      unfold AND OR,
+      simp,
+      rw eq_comm,
+    }
+  end
+
+--Complete circuit
+def SeqRecAux {n : ℕ} (X : signal) : Π (i : ℕ), i ≤ n → bool → bool → bool → ℕ → bool
+  |(nat.zero) h Q1 Q0 O k :=
+    if k ≤ 3 then
+      let Q1_next := LUT3 Q1 Q0 (X 0),
+          Q0_next := LUT2 Q1 Q0 (X 0),
+          O_next := LUT0 Q1_next Q0_next in
+      if O = tt then tt
+      else ff
+    else ff
+  |(nat.succ t) h Q1 Q0 O k :=
+    if k ≤ 3 then
+      let Q1_next := LUT3 Q1 Q0 (X t),
+          Q0_next := LUT2 Q1 Q0 (X t),
+          O_next := LUT0 Q1_next Q0_next in
+      if O = tt then tt
+      else if k = 3 then ff
+      else SeqRecAux (t) (le_of_lt h) Q1_next Q0_next (O_next) (k+1)
+    else ff
+
+def SeqRec (X : signal) : signal :=
+  λ n, SeqRecAux X (n) (le_refl _) ff ff ff 0
+
+def SeqRec_spec (X OUT : ℕ → bool) : Prop :=
+  ∀ t : ℕ, 
+    (X t = tt → X (t+1) = ff → X (t+2) = tt → OUT (t+3) = tt) ∧ 
+    (X t = ff → OUT (t+3) = ff)
+
+def SeqReq_correct : ∀ (X : ℕ → bool),
+  SeqRec_spec X (SeqRec X) :=
+  begin
+    intros X,
+    unfold SeqRec_spec,
+    intros t,
+    split,
+    {
+      intros h₁ h₂ h₃,
+      unfold SeqRec,
+      repeat {
+        unfold SeqRecAux,
+        simp,
+      },
+      unfold LUT0 LUT3 LUT2 OR AND,
+      simp,
+      unfold NOT,
+      simp,
+      rw h₃,
+      rw h₂,
+      simp,
+      unfold NOT,
+      simp,
+      rw h₁,
+      ring_nf,
+      simp,
+      cases t,
+      {
+        unfold SeqRecAux,
+        simp,
+      },
+      {
+        unfold SeqRecAux,
+        simp,
+      }
+    },
+    {
+      intro h₁,
+      unfold SeqRec,
+      repeat {
+        unfold SeqRecAux,
+        simp,
+      },
+      simp [LUT0, LUT2, LUT3, AND, OR, NOT],
+      cases X (t+1); cases X(t+2);
+      {
+        simp [NOT],
+        ring_nf,
+        simp,
+        cases t,
+        {
+          unfold SeqRecAux,
+          finish,
+        },
+        {
+          unfold SeqRecAux,
+          finish,
+        }
+      }
+    },
+  end
+
+--Example
+def X : signal := λx,x=0 ∨ x = 2 ∨ x = 4 ∨ x = 6 ∨ x=8 ∨ x=15 ∨ x = 17 
+#eval (SeqRec X) 
+
