src/Shifter.lean
@@ -1,0 +1,90 @@
+import Utility
+
+def shft_spec (A : array 4 bool) (D : bool) (OUT : array 4 bool) : Prop :=
+  if D = tt then OUT = ⟨λ i, if h : i.val > 0 ∧ i.val - 1 < 4 then A.read ⟨i.val - 1, h.right⟩ else ff⟩
+            else OUT = ⟨λ i, if h : i.val + 1 < 4 then A.read ⟨i.val + 1, h⟩ else ff⟩
+
+theorem shft_unique  : ∀ (A : array 4 bool) (D : bool),
+	∃! (OUT : array 4 bool), shft_spec A D OUT :=
+begin
+	intros A D,
+	apply exists_unique_of_exists_of_unique,
+	{
+    unfold shft_spec,
+    cases D;
+    {
+      exact exists_eq,
+    }
+	},
+	{
+		intros y₁ y₂,
+		unfold shft_spec,
+		intros h₁ h₂,
+    cases D;
+    {
+      simp at h₁ h₂,
+      rewrite ←h₂ at h₁,
+      exact h₁,
+    }
+	}
+end
+
+def shft_imp (A : array 4 bool) (D : bool) : array 4 bool :=
+  let D':= NOT D,
+      p := AND [A.read 0, D],
+      q := AND [D', A.read 1],
+      r := AND [D, A.read 1],
+      s := AND [D', A.read 2],
+      t := AND [D, A.read 2],
+      u := AND [D', A.read 3] in
+  [q, OR[p, s], OR[r, u], t].to_array
+
+
+theorem shft_correct : ∀ (A : array 4 bool) (D : bool) (OUT : array 4 bool),
+  shft_spec A D (shft_imp A D) :=
+  begin
+    intros A D OUT,
+    unfold shft_spec,
+    simp,
+    cases D;
+    {
+      simp,
+      unfold shft_imp,
+      apply array.ext,
+      intro i,
+      ring_nf,
+      unfold list.to_array,
+      dsimp at *,
+      unfold AND NOT OR,
+      simp,
+      cases i,
+      cases i_val with i_val₁,
+      {
+        refl,
+      },
+      {
+        cases i_val₁ with i_val₂,
+        {
+          refl,
+        },
+        {
+          cases i_val₂ with i_val₃,
+          {
+            refl,
+          },
+          {
+            cases i_val₃ with i_val₄,
+            {
+              refl,
+            },
+            {
+              exfalso,
+              repeat { rw nat.succ_eq_add_one at i_property },
+              simp at i_property,
+              exact i_property,
+            }
+          }
+        }
+      }
+    }
+  end
